cava/Cava/Monad/Combinators.v
@@ -330,20 +330,6 @@ Section WithCava.
     Vector.t A (2 ^ n) * Vector.t A (2 ^ n) :=
     splitat _ (@resize_default A (2 ^ (S n)) default (2 ^ n + 2 ^ n) v).
 
-  Fixpoint treeS {t: SignalType}
-                          {n : nat}
-                          (circuit: signal t -> signal t -> cava (signal t))
-                          (v : Vector.t (signal t) (2^(S n))) :
-                          cava (signal t) :=
-    match n, v return cava (signal t) with
-    | O, v2 => circuit (@Vector.nth_order _ 2 v2 0 (ltac:(lia)))
-                       (@Vector.nth_order _ 2 v2 1 (ltac:(lia)))
-    | S n', vR => let '(vL, vH) := divide defaultSignal vR in
-                  aS <- treeS circuit vL ;;
-                  bS <- treeS circuit vH ;;
-                  circuit aS bS
-    end.
-
   Fixpoint tree {T: Type} {m} `{Monad m}
                           (default : T) (n : nat)
                           (circuit: T -> T -> m T)
@@ -372,6 +358,15 @@ Section WithCava.
     rewrite resize_default_eq with (d0:=d).
     reflexivity.
   Qed.
+
+  (* A specialization of tree that is constrained to take Cava signal types
+    i.e. only types that we support as values over wires for Cava circuits.
+    This allows the default value to be computed automatically. *)
+  Definition treeS {t: SignalType} {n}
+                   (circuit: signal t * signal t -> cava (signal t))
+                   (v : Vector.t (signal t) (2^(S n))) :
+                   cava (signal t) :=
+  tree defaultSignal n (fun a b => circuit (a, b)) v.
 
   Local Open Scope nat_scope.
 
